backend/SCEV.v
@@ -1,0 +1,91 @@
+Require Import Coqlib Maps.
+Require Import AST Integers Values Events Memory Globalenvs Smallstep.
+Require Import Op Registers.
+Require Import AST.
+Require Import Cop.
+Require Import Cminor.
+Require Import Integers.
+Require Import Maps.
+
+Definition nat_to_int (n: nat): int := (Int.repr (Z.of_nat n)).
+Definition Z_to_int (z: Z): int := (Int.repr z).
+Definition z_to_val (z: Z) : val := Vint (Int.repr z).
+
+(* scev for identifier "i" that starts with first val and recurrences with val *)
+Inductive scev: Type :=
+  SCEVAddRec: Z -> Z -> scev.
+
+Definition numiters := positive.
+
+Fixpoint eval_scev (s: scev) (n: nat) : Z :=
+  match s with
+    | SCEVAddRec init step => match n with
+                             | 0%nat => init
+                             | S n' => step +  (eval_scev s n')
+                             end
+  end.
+
+
+
+
+Definition oned_loop (n: nat) (ivname: ident) (inner_stmt: Cminor.stmt): Cminor.stmt :=
+Sloop (
+    Sblock (
+        Cminor.Sseq (Sifthenelse (Ebinop
+                                    (Ocmp  Clt)
+                                    (Evar ivname)
+                                    (Econst (Ointconst (nat_to_int n))))
+                                 (Sskip)
+                                 (Sexit 1) (* this is a hack, there is no reason it has to be 0 *)
+                    )
+                    (inner_stmt)
+      )
+  ).
+
+Definition iv_init (ivname: ident) (iv_init_val: Z): Cminor.stmt :=
+  Sassign ivname (Econst (Ointconst (Int.repr iv_init_val))).
+
+
+Definition oned_loop_with_init (n: nat)
+           (ivname: ident)
+           (iv_init_val: Z)
+           (inner_stmt: Cminor.stmt): Cminor.stmt :=
+  Cminor.Sseq
+    (iv_init ivname iv_init_val)
+    (oned_loop n ivname inner_stmt).
+
+
+Definition oned_loop_add_rec (n: nat) (ivname: ident) (iv_init_val: Z) (add_val: Z) : Cminor.stmt :=
+  oned_loop_with_init n ivname iv_init_val
+            (Sassign
+               ivname
+               (Ebinop
+                  Oadd
+                  (Evar ivname)
+                  (Econst (Ointconst (Int.repr add_val))))).
+
+Lemma iv_init_sets_iv_value: forall (ivname: ident)
+                               (iv_init_val: Z),
+    
+   forall (m m': mem) (e e': env) (f: function) (sp: val) (ge: genv),
+    exec_stmt ge f sp e m
+              (iv_init ivname iv_init_val) E0
+              e' m' Out_normal -> e' ! ivname = Some (z_to_val iv_init_val).
+Abort.
+
+
+
+  
+
+(* Theorem on how a 1-D loop with match that of a SCEV Value *)
+Theorem oned_loop_add_rec_matches_addrec_scev:
+  forall (n: nat) (ivname: ident) (iv_init_val iv_add_val: Z),
+   forall (m m': mem) (e e': env) (f: function) (sp: val) (ge: genv),
+    exec_stmt ge f sp e m
+              (oned_loop_add_rec n ivname iv_init_val iv_add_val) E0
+              e' m' Out_normal ->
+    e' ! ivname =  Some (z_to_val (eval_scev (SCEVAddRec iv_init_val iv_add_val) n)).
+    
+    
+    
+Hint Transparent cm_loop_0_to_ub.
